Optimizations/Canonicalizations/AddPhase.thy
@@ -1,23 +1,7 @@
 theory AddPhase
   imports
-    OptimizationDSL.Canonicalization
-    "HOL-Eisbach.Eisbach"
+    Common
 begin
-
-fun size :: "IRExpr \<Rightarrow> nat" where
-  "size (UnaryExpr op e) = (size e) + 1" |
-  "size (BinaryExpr BinAdd x y) = (size x) + ((size y) * 2)" |
-  "size (BinaryExpr op x y) = (size x) + (size y)" |
-  "size (ConditionalExpr cond t f) = (size cond) + (size t) + (size f) + 2" |
-  "size (ConstantExpr c) = 1" |
-  "size (ParameterExpr ind s) = 2" |
-  "size (LeafExpr nid s) = 2" |
-  "size (ConstantVar c) = 2" |
-  "size (VariableExpr x s) = 2"
-
-method unfold_optimization =
-  (unfold rewrite_preservation.simps, unfold rewrite_termination.simps,
-    rule conjE, simp, simp del: le_expr_def)
 
 phase SnipPhase 
   trm size
