Optimizations/Canonicalizations/ConditionalPhase.thy
@@ -1,93 +1,57 @@
 theory ConditionalPhase
-  imports 
-    OptimizationDSL.Canonicalization
-    "HOL-Eisbach.Eisbach"
+  imports
+    Common
     Semantics.IRTreeEvalThms
+    Proofs.StampEvalThms
 begin
-
-fun size :: "IRExpr \<Rightarrow> nat" where
-  "size (UnaryExpr op e) = (size e) + 1" |
-  "size (BinaryExpr BinAdd x y) = (size x) + ((size y) * 2)" |
-  "size (BinaryExpr op x y) = (size x) + (size y)" |
-  "size (ConditionalExpr cond t f) = (size cond) + (size t) + (size f) + 2" |
-  "size (ConstantExpr c) = 1" |
-  "size (ParameterExpr ind s) = 2" |
-  "size (LeafExpr nid s) = 2" |
-  "size (ConstantVar c) = 2" |
-  "size (VariableExpr x s) = 2"
-
-method unfold_optimization =
-  (unfold rewrite_preservation.simps, unfold rewrite_termination.simps,
-    unfold intval.simps,
-    rule conjE, simp, simp del: le_expr_def)
-  | (unfold rewrite_preservation.simps, unfold rewrite_termination.simps,
-    rule conjE, simp, simp del: le_expr_def)
 
 phase Conditional
   trm size
 begin
 
-optimization a: "(e ? x : x) \<mapsto> x"
+lemma negates: "is_IntVal32 e \<or> is_IntVal64 e \<Longrightarrow> val_to_bool (val[e]) \<equiv> \<not>(val_to_bool (val[\<not>e]))"
+  by (smt (verit, best) Value.disc(1) Value.disc(10) Value.disc(4) Value.disc(5) Value.disc(6) Value.disc(9) intval_logic_negation.elims val_to_bool.simps(1) val_to_bool.simps(2) zero_neq_one)
+
+optimization negate_condition: "((\<not>e) ? x : y) \<mapsto> (e ? y : x)"
+    apply unfold_optimization
+  using negates evaltree.ConditionalExpr
+  apply (smt (verit, best) ConditionalExprE UnaryExprE is_IntVal32_def is_IntVal64_def le_expr_def stamp_implies_valid_value unary_eval.simps(4) valid_value.elims(2))
+  unfolding size.simps by simp
+
+optimization const_true: "((const(IntVal32 1)) ? x : y) \<mapsto> x"
+   apply unfold_optimization
+   apply force
+  unfolding size.simps by simp
+
+optimization const_false: "((const(IntVal32 0)) ? x : y) \<mapsto> y"
+   apply unfold_optimization
+   apply force
+  unfolding size.simps by simp
+
+optimization equal_branches: "(e ? x : x) \<mapsto> x"
    apply unfold_optimization
    apply force
   unfolding size.simps by auto
 
+optimization condition_bounds_x: "((x < y) ? x : y) \<mapsto> x when stamp_under (stamp_expr x) (stamp_expr y)"
+   apply unfold_optimization
+  using stamp_under_semantics
+   apply fastforce
+  unfolding size.simps by simp
+
+optimization condition_bounds_y: "((x < y) ? x : y) \<mapsto> y when stamp_under (stamp_expr y) (stamp_expr x)"
+   apply unfold_optimization
+  using stamp_under_semantics_inversed
+   apply fastforce
+  unfolding size.simps by simp
+
+(*extra one*)
 optimization b[intval]: "((x eq y) ? x : y) \<mapsto> y"
    apply unfold_optimization
     apply (smt (z3) bool_to_val.simps(2) intval_equals.elims val_to_bool.simps(1) val_to_bool.simps(3))
     unfolding intval.simps
     apply (smt (z3) BinaryExprE ConditionalExprE Value.inject(1) Value.inject(2) bin_eval.simps(10) bool_to_val.simps(2) evalDet intval_equals.simps(1) intval_equals.simps(10) intval_equals.simps(12) intval_equals.simps(15) intval_equals.simps(16) intval_equals.simps(2) intval_equals.simps(5) intval_equals.simps(8) intval_equals.simps(9) le_expr_def val_to_bool.cases val_to_bool.elims(2))
   unfolding size.simps by auto
-
-(*
-lemma unary_eval_outcome: 
-  "is_IntVal32 (unary_eval op e) \<or> is_IntVal64 (unary_eval op e) \<or> (unary_eval op e) = UndefVal"
-  apply (cases op; auto)
-     apply (metis Value.exhaust_sel intval_abs.simps(1) intval_abs.simps(2) intval_abs.simps(3) intval_abs.simps(4) intval_abs.simps(5) is_IntVal32_def is_IntVal64_def)
-    apply (metis intval_negate.elims is_IntVal32_def is_IntVal64_def)
-   apply (metis intval_not.elims is_IntVal32_def is_IntVal64_def)
-  by (metis Value.exhaust_sel intval_logic_negation.simps(1) intval_logic_negation.simps(2) intval_logic_negation.simps(3) intval_logic_negation.simps(4) intval_logic_negation.simps(5) is_IntVal32_def is_IntVal64_def)
-
-lemma valid_under: "[m, p] \<turnstile> e \<mapsto> v \<Longrightarrow> valid_value (stamp_expr e) v"
-  sorry
-
-lemma "stamp_under x y 
-      \<Longrightarrow> [m, p] \<turnstile> x \<mapsto> e1 \<and> [m, p] \<turnstile> y \<mapsto> e2 
-      \<Longrightarrow> val_to_bool (intval_less_than e1 e2)"
-  using valid_under sorry
-*)
-
-fun stamp_under :: "IRExpr \<Rightarrow> IRExpr \<Rightarrow> bool" where
-  "stamp_under x y = (stpi_upper (stamp_expr x) < stpi_lower (stamp_expr y))"
-
-(* The problem:
-   Stamps aren't required to be correct in the evaluation semantics yet.
-*)
-optimization c: "((x < y) ? x : y) \<mapsto> x when stamp_under x y"
-   apply unfold_optimization
-  sorry
-
-
-lemma negates: "is_IntVal32 e \<or> is_IntVal64 e \<Longrightarrow> val_to_bool (val[e]) \<equiv> \<not>(val_to_bool (val[\<not>e]))"
-  by (smt (verit, best) Value.disc(1) Value.disc(10) Value.disc(4) Value.disc(5) Value.disc(6) Value.disc(9) intval_logic_negation.elims val_to_bool.simps(1) val_to_bool.simps(2) zero_neq_one)
-
-(* The problem:
-   Evaluation of e and \<not>e needs to be of IntVal32 or IntVal64 to allow the above lemma
-   to be used. I haven't yet found a way to show this.
-*)
-optimization d[intval]: "((\<not>e) ? x : y) \<mapsto> (e ? y : x)"
-    apply unfold_optimization
-  using negates sorry 
-
-optimization e: "((const(IntVal32 1)) ? x : y) \<mapsto> x"
-   apply unfold_optimization
-   apply force
-  unfolding size.simps by simp
-
-optimization f: "((const(IntVal32 0)) ? x : y) \<mapsto> y"
-   apply unfold_optimization
-   apply force
-  unfolding size.simps by simp
 
 end
 
