Proofs/StampEvalThms.thy
@@ -1,0 +1,504 @@
+theory StampEvalThms
+  imports Semantics.IRTreeEvalThms
+begin
+
+(* these two were weirdly hard to prove given it should be by definition *)
+lemma size32: "size v = 32" for v :: "32 word"
+  using size_word.rep_eq
+  using One_nat_def add.right_neutral add_Suc_right len_of_numeral_defs(2) len_of_numeral_defs(3) mult.right_neutral mult_Suc_right numeral_2_eq_2 numeral_Bit0
+  by (smt (verit, del_insts) mult.commute)
+
+lemma size64: "size v = 64" for v :: "64 word"
+  using size_word.rep_eq
+  using One_nat_def add.right_neutral add_Suc_right len_of_numeral_defs(2) len_of_numeral_defs(3) mult.right_neutral mult_Suc_right numeral_2_eq_2 numeral_Bit0
+  by (smt (verit, del_insts) mult.commute)
+
+lemma signed_int_bottom32: "-(((2::int) ^ 31)) \<le> sint (v::int32)"
+  using sint_range_size size32
+  by (smt (verit, ccfv_SIG) One_nat_def Suc_pred add_Suc add_Suc_right eval_nat_numeral(3) nat.inject numeral_2_eq_2 numeral_Bit0 numeral_Bit1 zero_less_numeral)
+
+lemma signed_int_top32: "(2 ^ 31) - 1 \<ge> sint (v::int32)"
+  using sint_range_size size32
+  by (smt (verit, ccfv_SIG) One_nat_def Suc_pred add_Suc add_Suc_right eval_nat_numeral(3) nat.inject numeral_2_eq_2 numeral_Bit0 numeral_Bit1 zero_less_numeral)
+
+lemma lower_bounds_equiv32: "-(((2::int) ^ 31)) = (2::int) ^ 32 div 2 * - 1"
+  by fastforce
+
+lemma upper_bounds_equiv32: "(2::int) ^ 31 = (2::int) ^ 32 div 2"
+  by simp
+
+lemma bit_bounds_min32: "((fst (bit_bounds 32))) \<le> (sint (v::int32))"
+  unfolding bit_bounds.simps fst_def using signed_int_bottom32 lower_bounds_equiv32
+  by auto
+
+lemma bit_bounds_max32: "((snd (bit_bounds 32))) \<ge> (sint (v::int32))"
+  unfolding bit_bounds.simps fst_def using signed_int_top32 upper_bounds_equiv32
+  by auto
+
+lemma signed_int_bottom64: "-(((2::int) ^ 63)) \<le> sint (v::int64)"
+  using sint_range_size size64
+  by (smt (verit, ccfv_SIG) One_nat_def Suc_pred add_Suc add_Suc_right eval_nat_numeral(3) nat.inject numeral_2_eq_2 numeral_Bit0 numeral_Bit1 zero_less_numeral)
+
+lemma signed_int_top64: "(2 ^ 63) - 1 \<ge> sint (v::int64)"
+  using sint_range_size size64
+  by (smt (verit, ccfv_SIG) One_nat_def Suc_pred add_Suc add_Suc_right eval_nat_numeral(3) nat.inject numeral_2_eq_2 numeral_Bit0 numeral_Bit1 zero_less_numeral)
+
+lemma lower_bounds_equiv64: "-(((2::int) ^ 63)) = (2::int) ^ 64 div 2 * - 1"
+  by fastforce
+
+lemma upper_bounds_equiv64: "(2::int) ^ 63 = (2::int) ^ 64 div 2"
+  by simp
+
+lemma bit_bounds_min64: "((fst (bit_bounds 64))) \<le> (sint (v::int64))"
+  unfolding bit_bounds.simps fst_def using signed_int_bottom64 lower_bounds_equiv64
+  by auto
+
+lemma bit_bounds_max64: "((snd (bit_bounds 64))) \<ge> (sint (v::int64))"
+  unfolding bit_bounds.simps fst_def using signed_int_top64 upper_bounds_equiv64
+  by auto
+
+lemma unrestricted_32bit_always_valid:
+  "valid_value (IntVal32 v) (unrestricted_stamp (IntegerStamp 32 lo hi))"
+  using valid_value.simps(1) bit_bounds_min32 bit_bounds_max32
+  using unrestricted_stamp.simps(2) by presburger
+
+lemma unrestricted_64bit_always_valid:
+  "valid_value (IntVal64 v) (unrestricted_stamp (IntegerStamp 64 lo hi))"
+  using valid_value.simps(2) bit_bounds_min64 bit_bounds_max64
+  using unrestricted_stamp.simps(2) by presburger
+
+lemma unary_undef: "val = UndefVal \<Longrightarrow> unary_eval op val = UndefVal"
+  by (cases op; auto)
+
+lemma unary_obj: "val = ObjRef x \<Longrightarrow> unary_eval op val = UndefVal"
+  by (cases op; auto)
+
+lemma unary_eval_implies_valud_value:
+  assumes "[m,p] \<turnstile> expr \<mapsto> val"
+  assumes "result = unary_eval op val"
+  assumes "result \<noteq> UndefVal"
+  assumes "valid_value val (stamp_expr expr)"
+  shows "valid_value result (stamp_expr (UnaryExpr op expr))"
+proof -
+  have is_IntVal: "\<exists> x y. result = IntVal32 x \<or> result = IntVal64 y"
+    using assms(2,3) apply (cases op; auto; cases val; auto)
+    apply metis
+    by metis
+  then have "is_IntegerStamp (stamp_expr expr)"
+    using assms(2,3,4) apply (cases "(stamp_expr expr)"; auto) 
+    using valid_VoidStamp unary_undef apply simp
+    using valid_VoidStamp unary_undef apply simp
+    using valid_ObjStamp unary_obj apply fastforce
+    using valid_ObjStamp unary_obj by fastforce
+  then obtain b lo hi where stamp_expr_def: "stamp_expr expr = (IntegerStamp b lo hi)"
+    using is_IntegerStamp_def by auto
+  then have "stamp_expr (UnaryExpr op expr) = unrestricted_stamp (IntegerStamp b lo hi)"
+    using stamp_expr.simps(1) stamp_unary.simps(1) by presburger
+  from stamp_expr_def have bit32: "b = 32 \<Longrightarrow> \<exists> x. result = IntVal32 x"
+    using assms(2,3,4) by (cases op; auto; cases val; auto) 
+  from stamp_expr_def have bit64: "b = 64 \<Longrightarrow> \<exists> x. result = IntVal64 x" 
+    using assms(2,3,4) by (cases op; auto; cases val; auto) 
+
+  show ?thesis using valid_value.simps(1,2)
+    unrestricted_32bit_always_valid unrestricted_64bit_always_valid stamp_expr_def
+    bit32 bit64
+    by (metis \<open>stamp_expr (UnaryExpr op expr) = unrestricted_stamp (IntegerStamp b lo hi)\<close> assms(4) valid32or64_both)
+qed
+
+lemma binary_undef: "v1 = UndefVal \<or> v2 = UndefVal \<Longrightarrow> bin_eval op v1 v2 = UndefVal"
+  by (cases op; auto)
+
+lemma binary_obj: "v1 = ObjRef x \<or> v2 = ObjRef y \<Longrightarrow> bin_eval op v1 v2 = UndefVal"
+  by (cases op; auto)
+
+lemma binary_eval_bits_equal:
+  assumes "result = bin_eval op val1 val2"
+  assumes "result \<noteq> UndefVal"
+  assumes "valid_value val1 (IntegerStamp b1 lo1 hi1)"
+  assumes "valid_value val2 (IntegerStamp b2 lo2 hi2)"
+  shows "b1 = b2"
+  using assms 
+  by (cases op; cases val1; cases val2; auto) (*slow*)
+
+lemma binary_eval_values:
+  assumes "\<exists>x y. result = IntVal32 x \<or> result = IntVal64 y"
+  assumes "result = bin_eval op val1 val2"
+  shows" \<exists>x32 x64 y32 y64. val1 = IntVal32 x32 \<and> val2 = IntVal32 y32 \<or> val1 = IntVal64 x64 \<and> val2 = IntVal64 y64"
+  using assms apply (cases result)
+      apply simp apply (cases op; cases val1; cases val2; auto)
+    apply (cases op; cases val1; cases val2; auto) by auto+
+
+lemma binary_eval_implies_valud_value:
+  assumes "[m,p] \<turnstile> expr1 \<mapsto> val1"
+  assumes "[m,p] \<turnstile> expr2 \<mapsto> val2"
+  assumes "result = bin_eval op val1 val2"
+  assumes "result \<noteq> UndefVal"
+  assumes "valid_value val1 (stamp_expr expr1)"
+  assumes "valid_value val2 (stamp_expr expr2)"
+  shows "valid_value result (stamp_expr (BinaryExpr op expr1 expr2))"
+proof -
+  have is_IntVal: "\<exists> x y. result = IntVal32 x \<or> result = IntVal64 y"
+    using assms(1,2,3,4) apply (cases op; auto; cases val1; auto; cases val2; auto)
+    by (meson Values.bool_to_val.elims)+
+  then have expr1_intstamp: "is_IntegerStamp (stamp_expr expr1)"
+    using assms(1,3,4,5) apply (cases "(stamp_expr expr1)"; auto simp: valid_VoidStamp binary_undef)
+    using valid_ObjStamp binary_obj apply (metis assms(4))
+    using valid_ObjStamp binary_obj by (metis assms(4))
+  from is_IntVal have expr2_intstamp: "is_IntegerStamp (stamp_expr expr2)"
+    using assms(2,3,4,6) apply (cases "(stamp_expr expr2)"; auto simp: valid_VoidStamp binary_undef)
+    using valid_ObjStamp binary_obj apply (metis assms(4))
+    using valid_ObjStamp binary_obj by (metis assms(4))
+  from expr1_intstamp obtain b1 lo1 hi1 where stamp_expr1_def: "stamp_expr expr1 = (IntegerStamp b1 lo1 hi1)"
+    using is_IntegerStamp_def by auto
+  from expr2_intstamp obtain b2 lo2 hi2 where stamp_expr2_def: "stamp_expr expr2 = (IntegerStamp b2 lo2 hi2)"
+    using is_IntegerStamp_def by auto
+
+  have "\<exists> x32 x64 y32 y64 . (val1 = IntVal32 x32 \<and> val2 = IntVal32 y32) \<or> (val1 = IntVal64 x64 \<and> val2 = IntVal64 y64)"
+    using is_IntVal assms(3) binary_eval_values
+    by presburger
+    
+  have "b1 = b2"
+    using assms(3,4,5,6) stamp_expr1_def stamp_expr2_def
+    using binary_eval_bits_equal
+    by auto 
+  then have stamp_def: "stamp_expr (BinaryExpr op expr1 expr2) = 
+    (case op \<in> fixed_32 of True \<Rightarrow> unrestricted_stamp (IntegerStamp 32 lo1 hi1)| False \<Rightarrow> unrestricted_stamp (IntegerStamp b1 lo1 hi1))"
+    using stamp_expr.simps(2) stamp_binary.simps(1)
+    using stamp_expr1_def stamp_expr2_def by presburger
+  from stamp_expr1_def have bit32: "b1 = 32 \<Longrightarrow> \<exists> x. result = IntVal32 x"
+    using assms apply (cases op; cases val1; cases val2; auto) (*slow*)
+    by (meson Values.bool_to_val.elims)+
+  from stamp_expr1_def have bit64: "b1 = 64 \<and> op \<notin> fixed_32 \<Longrightarrow> \<exists> x y. result = IntVal64 x" 
+    using assms apply (cases op; cases val1; cases val2; simp) (*slow*)
+    using fixed_32_def by auto+
+  from stamp_expr1_def have fixed: "op \<in> fixed_32 \<Longrightarrow> \<exists> x y. result = IntVal32 x" 
+    using assms unfolding fixed_32_def apply (cases op; auto)
+    apply (cases val1; cases val2; auto)
+    using bit32 apply fastforce 
+      apply (meson Values.bool_to_val.elims)
+     apply (cases val1; cases val2; auto) 
+    using bit32 apply fastforce
+     apply (meson Values.bool_to_val.elims)
+      apply (cases val1; cases val2; auto) 
+    using bit32 apply fastforce
+    by (meson Values.bool_to_val.elims)
+
+  show ?thesis apply (cases "op \<in> fixed_32") defer using valid_value.simps(1,2)
+    unrestricted_32bit_always_valid unrestricted_64bit_always_valid stamp_expr1_def
+    bit32 bit64 stamp_def apply auto
+    using \<open>\<exists>x32 x64 y32 y64. val1 = IntVal32 x32 \<and> val2 = IntVal32 y32 \<or> val1 = IntVal64 x64 \<and> val2 = IntVal64 y64\<close> assms(5) apply auto[1]
+    using fixed by force
+qed
+
+lemma stamp_meet_is_valid:
+  assumes "valid_value val stamp1 \<or> valid_value val stamp2"
+  assumes "meet stamp1 stamp2 \<noteq> IllegalStamp"
+  shows "valid_value val (meet stamp1 stamp2)"
+  using assms proof (cases stamp1)
+  case VoidStamp
+  then show ?thesis
+    by (metis Stamp.exhaust assms(1) assms(2) meet.simps(1) meet.simps(37) meet.simps(44) meet.simps(51) meet.simps(58) meet.simps(65) meet.simps(66) meet.simps(67))
+next
+  case (IntegerStamp b lo hi)
+  obtain b2 lo2 hi2 where stamp2_def: "stamp2 = IntegerStamp b2 lo2 hi2"
+    by (metis IntegerStamp assms(2) meet.simps(45) meet.simps(52) meet.simps(59) meet.simps(6) meet.simps(65) meet.simps(66) meet.simps(67) unrestricted_stamp.cases)
+  then have "b = b2" using meet.simps(2) assms(2) 
+    by (metis IntegerStamp)
+  then have meet_def: "meet stamp1 stamp2 = (IntegerStamp b (min lo lo2) (max hi hi2))"
+    by (simp add: IntegerStamp stamp2_def)
+  then show ?thesis proof (cases "b = 32")
+    case True
+    then obtain x where val_def: "val = IntVal32 x"
+      using IntegerStamp assms(1) valid32
+      using \<open>b = b2\<close> stamp2_def by blast
+    have min: "sint x \<ge> min lo lo2" 
+      using val_def
+      using IntegerStamp assms(1)
+      using stamp2_def by force
+    have max: "sint x \<le> max hi hi2" 
+      using val_def
+      using IntegerStamp assms(1)
+      using stamp2_def by force
+    from min max show ?thesis
+      by (simp add: True meet_def val_def)
+  next
+    case False
+    then have bit64: "b = 64"
+      using assms(1) IntegerStamp valid_value.simps
+      valid32or64_both
+      by (metis \<open>b = b2\<close> stamp2_def)
+    then obtain x where val_def: "val = IntVal64 x"
+      using IntegerStamp assms(1) valid64
+      using \<open>b = b2\<close> stamp2_def by blast
+    have min: "sint x \<ge> min lo lo2" 
+      using val_def
+      using IntegerStamp assms(1)
+      using stamp2_def by force
+    have max: "sint x \<le> max hi hi2" 
+      using val_def
+      using IntegerStamp assms(1)
+      using stamp2_def by force
+    from min max show ?thesis
+      by (simp add: bit64 meet_def val_def)
+  qed
+next
+  case (KlassPointerStamp x31 x32)
+  then show ?thesis using assms valid_value.elims(2)
+    by (metis meet.simps(14) valid_value.simps(21))
+next
+  case (MethodCountersPointerStamp x41 x42)
+  then show ?thesis using assms valid_value.elims(2)
+    by (metis meet.simps(39) valid_value.simps(22))
+next
+  case (MethodPointersStamp x51 x52)
+then show ?thesis using assms valid_value.elims(2)
+  by (metis meet.simps(40) valid_value.simps(23))
+next
+  case (ObjectStamp x61 x62 x63 x64)
+  then show ?thesis using assms
+    using meet.simps(34) by blast
+next
+  case (RawPointerStamp x71 x72)
+  then show ?thesis using assms
+    using meet.simps(35) by blast
+next
+  case IllegalStamp
+  then show ?thesis using assms
+    using meet.simps(36) by blast
+qed
+
+
+lemma conditional_eval_implies_valud_value:
+  assumes "[m,p] \<turnstile> cond \<mapsto> condv"
+  assumes "expr = (if val_to_bool condv then expr1 else expr2)"
+  assumes "[m,p] \<turnstile> expr \<mapsto> val"
+  assumes "val \<noteq> UndefVal"
+  assumes "valid_value condv (stamp_expr cond)"
+  assumes "valid_value val (stamp_expr expr)"
+  shows "valid_value val (stamp_expr (ConditionalExpr cond expr1 expr2))"
+proof -
+  have "meet (stamp_expr expr1) (stamp_expr expr2) \<noteq> IllegalStamp"
+    using assms apply (cases "stamp_expr expr"; auto)
+    using valid_VoidStamp sorry
+  then show ?thesis using stamp_meet_is_valid using stamp_expr.simps(6)
+    using assms(2) assms(6) by presburger
+qed
+
+lemma stamp_implies_valid_value:
+  assumes "[m,p] \<turnstile> expr \<mapsto> val"
+  shows "valid_value val (stamp_expr expr)"
+  using assms proof (induction expr val)
+case (UnaryExpr expr val result op)
+  then show ?case using unary_eval_implies_valud_value by simp
+next
+  case (BinaryExpr expr1 val1 expr2 val2 result op)
+  then show ?case using binary_eval_implies_valud_value by simp
+next
+  case (ConditionalExpr cond condv expr expr1 expr2 val)
+  then show ?case using conditional_eval_implies_valud_value by simp
+next
+  case (ParameterExpr x1 x2)
+  then show ?case by auto
+next
+  case (LeafExpr x1 x2)
+  then show ?case by auto
+next
+  case (ConstantExpr x)
+  then show ?case by auto
+qed
+
+
+lemma value_range:
+  assumes "[m, p] \<turnstile> e \<mapsto> v"
+  shows "v \<in> {val . valid_value val (stamp_expr e)}"
+  using assms stamp_implies_valid_value
+  by simp
+
+lemma upper_bound_32:
+  assumes "val = IntVal32 v"
+  assumes "\<exists> l h. s = (IntegerStamp 32 l h)"
+  shows "valid_value val s \<Longrightarrow> sint v \<le> (stpi_upper s)"
+  using assms by force
+
+lemma upper_bound_64:
+  assumes "val = IntVal64 v"
+  assumes "\<exists> l h. s = (IntegerStamp 64 l h)"
+  shows "valid_value val s \<Longrightarrow> sint v \<le> (stpi_upper s)"
+  using assms by force
+
+lemma lower_bound_32:
+  assumes "val = IntVal32 v"
+  assumes "\<exists> l h. s = (IntegerStamp 32 l h)"
+  shows "valid_value val s \<Longrightarrow> sint v \<ge> (stpi_lower s)"
+  using assms by force
+
+lemma lower_bound_64:
+  assumes "val = IntVal64 v"
+  assumes "\<exists> l h. s = (IntegerStamp 64 l h)"
+  shows "valid_value val s \<Longrightarrow> sint v \<ge> (stpi_lower s)"
+  using assms
+  by force
+
+
+(* these two proofs should really not be so tricky *)
+lemma stamp_under_semantics:
+  assumes "stamp_under (stamp_expr x) (stamp_expr y)"
+  assumes "[m, p] \<turnstile> (BinaryExpr BinIntegerLessThan x y) \<mapsto> v"
+  shows "val_to_bool v"
+proof -
+  obtain xval where xval_def: "[m, p] \<turnstile> x \<mapsto> xval"
+    using assms(2) by blast
+  obtain yval where yval_def: "[m, p] \<turnstile> y \<mapsto> yval"
+    using assms(2) by blast
+  have "is_IntVal32 xval \<or> is_IntVal64 xval"
+    by (metis is_IntVal32_def is_IntVal64_def stamp_implies_valid_value valid_value.elims(2) xval_def)
+  have "is_IntVal32 yval \<or> is_IntVal64 yval"
+    by (metis is_IntVal32_def is_IntVal64_def stamp_implies_valid_value valid_value.elims(2) yval_def)
+  have "is_IntVal32 xval = is_IntVal32 yval"
+    by (metis BinaryExprE Value.collapse(2) \<open>is_IntVal32 xval \<or> is_IntVal64 xval\<close> \<open>is_IntVal32 yval \<or> is_IntVal64 yval\<close> assms(2) bin_eval.simps(11) evalDet intval_less_than.simps(12) intval_less_than.simps(5) is_IntVal32_def xval_def yval_def)
+  have "is_IntVal64 xval = is_IntVal64 yval"
+    using \<open>is_IntVal32 xval = is_IntVal32 yval\<close> \<open>is_IntVal32 xval \<or> is_IntVal64 xval\<close> \<open>is_IntVal32 yval \<or> is_IntVal64 yval\<close> by blast
+  have "(intval_less_than xval yval) \<noteq> UndefVal"
+    using assms(2)
+    by (metis BinaryExprE bin_eval.simps(11) evalDet xval_def yval_def)
+  have "is_IntVal32 xval \<Longrightarrow> ((\<exists> lo hi. stamp_expr x = IntegerStamp 32 lo hi) \<and> (\<exists> lo hi. stamp_expr y = IntegerStamp 32 lo hi))"
+    by (smt (verit) BinaryExprE Value.discI(2) Value.distinct_disc(9) assms(2) binary_eval_bits_equal stamp_implies_valid_value valid_value.elims(2) xval_def)
+  have "is_IntVal64 xval \<Longrightarrow> ((\<exists> lo hi. stamp_expr x = IntegerStamp 64 lo hi) \<and> (\<exists> lo hi. stamp_expr y = IntegerStamp 64 lo hi))"
+    by (smt (verit, best) BinaryExprE \<open>intval_less_than xval yval \<noteq> UndefVal\<close> assms(2) binary_eval_bits_equal intval_less_than.simps(5) is_IntVal64_def stamp_implies_valid_value valid_value.elims(2) yval_def)
+  have xvalid: "valid_value xval (stamp_expr x)"
+    using stamp_implies_valid_value xval_def by auto
+  have yvalid: "valid_value yval (stamp_expr y)"
+    using stamp_implies_valid_value yval_def by auto
+  { assume c: "is_IntVal32 xval"
+    obtain xxval where x32: "xval = IntVal32 xxval"
+      using c is_IntVal32_def by blast
+    obtain yyval where y32: "yval = IntVal32 yyval"
+      using \<open>is_IntVal32 xval = is_IntVal32 yval\<close> c is_IntVal32_def by auto
+    have xs: "\<exists> lo hi. stamp_expr x = IntegerStamp 32 lo hi"
+      by (simp add: \<open>is_IntVal32 xval \<Longrightarrow> (\<exists>lo hi. stamp_expr x = IntegerStamp 32 lo hi) \<and> (\<exists>lo hi. stamp_expr y = IntegerStamp 32 lo hi)\<close> c)
+    have ys: "\<exists> lo hi. stamp_expr y = IntegerStamp 32 lo hi"
+      using \<open>is_IntVal32 xval \<Longrightarrow> (\<exists>lo hi. stamp_expr x = IntegerStamp 32 lo hi) \<and> (\<exists>lo hi. stamp_expr y = IntegerStamp 32 lo hi)\<close> c by blast
+    have "sint xxval \<le> stpi_upper (stamp_expr x)"
+      using upper_bound_32 x32 xs xvalid by presburger
+    have "stpi_lower (stamp_expr y) \<le> sint yyval"
+      using lower_bound_32 y32 ys yvalid by presburger
+    have "stpi_upper (stamp_expr x) < stpi_lower (stamp_expr y)"
+      using assms(1) unfolding stamp_under.simps
+      by auto
+    then have "xxval <s yyval"
+      using assms(1) unfolding stamp_under.simps
+      using \<open>sint xxval \<sqsubseteq> stpi_upper (stamp_expr x)\<close> \<open>stpi_lower (stamp_expr y) \<sqsubseteq> sint yyval\<close> word_sless_alt by fastforce
+    then have "(intval_less_than xval yval) = IntVal32 1"
+      by (simp add: x32 y32)
+  }
+  note case32 = this
+  { assume c: "is_IntVal64 xval"
+    obtain xxval where x64: "xval = IntVal64 xxval"
+      using c is_IntVal64_def by blast
+    obtain yyval where y64: "yval = IntVal64 yyval"
+      using \<open>is_IntVal64 xval = is_IntVal64 yval\<close> c is_IntVal64_def by auto
+    have xs: "\<exists> lo hi. stamp_expr x = IntegerStamp 64 lo hi"
+      by (simp add: \<open>is_IntVal64 xval \<Longrightarrow> (\<exists>lo hi. stamp_expr x = IntegerStamp 64 lo hi) \<and> (\<exists>lo hi. stamp_expr y = IntegerStamp 64 lo hi)\<close> c)
+    have ys: "\<exists> lo hi. stamp_expr y = IntegerStamp 64 lo hi"
+      using \<open>is_IntVal64 xval \<Longrightarrow> (\<exists>lo hi. stamp_expr x = IntegerStamp 64 lo hi) \<and> (\<exists>lo hi. stamp_expr y = IntegerStamp 64 lo hi)\<close> c by blast
+    have "sint xxval \<le> stpi_upper (stamp_expr x)"
+      using upper_bound_64 x64 xs xvalid by presburger
+    have "stpi_lower (stamp_expr y) \<le> sint yyval"
+      using lower_bound_64 y64 ys yvalid by presburger
+    have "stpi_upper (stamp_expr x) < stpi_lower (stamp_expr y)"
+      using assms(1) unfolding stamp_under.simps
+      by auto
+    then have "xxval <s yyval"
+      using assms(1) unfolding stamp_under.simps
+      using \<open>sint xxval \<sqsubseteq> stpi_upper (stamp_expr x)\<close> \<open>stpi_lower (stamp_expr y) \<sqsubseteq> sint yyval\<close> word_sless_alt by fastforce
+    then have "(intval_less_than xval yval) = IntVal32 1"
+      by (simp add: x64 y64)
+  }
+  note case64 = this
+  have "(intval_less_than xval yval) = IntVal32 1"
+    using \<open>is_IntVal32 xval \<or> is_IntVal64 xval\<close> case32 case64 by fastforce
+  then show ?thesis
+    by (metis BinaryExprE assms(2) bin_eval.simps(11) evalDet val_to_bool.simps(1) xval_def yval_def zero_neq_one)
+qed
+
+lemma stamp_under_semantics_inversed:
+  assumes "stamp_under (stamp_expr y) (stamp_expr x)"
+  assumes "[m, p] \<turnstile> (BinaryExpr BinIntegerLessThan x y) \<mapsto> v"
+  shows "\<not>(val_to_bool v)"
+proof -
+  obtain xval where xval_def: "[m, p] \<turnstile> x \<mapsto> xval"
+    using assms(2) by blast
+  obtain yval where yval_def: "[m, p] \<turnstile> y \<mapsto> yval"
+    using assms(2) by blast
+  have "is_IntVal32 xval \<or> is_IntVal64 xval"
+    by (metis is_IntVal32_def is_IntVal64_def stamp_implies_valid_value valid_value.elims(2) xval_def)
+  have "is_IntVal32 yval \<or> is_IntVal64 yval"
+    by (metis is_IntVal32_def is_IntVal64_def stamp_implies_valid_value valid_value.elims(2) yval_def)
+  have "is_IntVal32 xval = is_IntVal32 yval"
+    by (metis BinaryExprE Value.collapse(2) \<open>is_IntVal32 xval \<or> is_IntVal64 xval\<close> \<open>is_IntVal32 yval \<or> is_IntVal64 yval\<close> assms(2) bin_eval.simps(11) evalDet intval_less_than.simps(12) intval_less_than.simps(5) is_IntVal32_def xval_def yval_def)
+  have "is_IntVal64 xval = is_IntVal64 yval"
+    using \<open>is_IntVal32 xval = is_IntVal32 yval\<close> \<open>is_IntVal32 xval \<or> is_IntVal64 xval\<close> \<open>is_IntVal32 yval \<or> is_IntVal64 yval\<close> by blast
+  have "(intval_less_than xval yval) \<noteq> UndefVal"
+    using assms(2)
+    by (metis BinaryExprE bin_eval.simps(11) evalDet xval_def yval_def)
+  have "is_IntVal32 xval \<Longrightarrow> ((\<exists> lo hi. stamp_expr x = IntegerStamp 32 lo hi) \<and> (\<exists> lo hi. stamp_expr y = IntegerStamp 32 lo hi))"
+    by (smt (verit) BinaryExprE Value.discI(2) Value.distinct_disc(9) assms(2) binary_eval_bits_equal stamp_implies_valid_value valid_value.elims(2) xval_def)
+  have "is_IntVal64 xval \<Longrightarrow> ((\<exists> lo hi. stamp_expr x = IntegerStamp 64 lo hi) \<and> (\<exists> lo hi. stamp_expr y = IntegerStamp 64 lo hi))"
+    by (smt (verit, best) BinaryExprE \<open>intval_less_than xval yval \<noteq> UndefVal\<close> assms(2) binary_eval_bits_equal intval_less_than.simps(5) is_IntVal64_def stamp_implies_valid_value valid_value.elims(2) yval_def)
+  have xvalid: "valid_value xval (stamp_expr x)"
+    using stamp_implies_valid_value xval_def by auto
+  have yvalid: "valid_value yval (stamp_expr y)"
+    using stamp_implies_valid_value yval_def by auto
+  { assume c: "is_IntVal32 xval"
+    obtain xxval where x32: "xval = IntVal32 xxval"
+      using c is_IntVal32_def by blast
+    obtain yyval where y32: "yval = IntVal32 yyval"
+      using \<open>is_IntVal32 xval = is_IntVal32 yval\<close> c is_IntVal32_def by auto
+    have xs: "\<exists> lo hi. stamp_expr x = IntegerStamp 32 lo hi"
+      by (simp add: \<open>is_IntVal32 xval \<Longrightarrow> (\<exists>lo hi. stamp_expr x = IntegerStamp 32 lo hi) \<and> (\<exists>lo hi. stamp_expr y = IntegerStamp 32 lo hi)\<close> c)
+    have ys: "\<exists> lo hi. stamp_expr y = IntegerStamp 32 lo hi"
+      using \<open>is_IntVal32 xval \<Longrightarrow> (\<exists>lo hi. stamp_expr x = IntegerStamp 32 lo hi) \<and> (\<exists>lo hi. stamp_expr y = IntegerStamp 32 lo hi)\<close> c by blast
+    have "sint yyval \<le> stpi_upper (stamp_expr y)"
+      using y32 ys yvalid by force
+    have "stpi_lower (stamp_expr x) \<le> sint xxval"
+      using x32 xs xvalid by force
+    have "stpi_upper (stamp_expr y) < stpi_lower (stamp_expr x)"
+      using assms(1) unfolding stamp_under.simps
+      by auto
+    then have "yyval <s xxval"
+      using assms(1) unfolding stamp_under.simps
+      using \<open>sint yyval \<sqsubseteq> stpi_upper (stamp_expr y)\<close> \<open>stpi_lower (stamp_expr x) \<sqsubseteq> sint xxval\<close> word_sless_alt by fastforce
+    then have "(intval_less_than xval yval) = IntVal32 0"
+      using signed.less_not_sym x32 y32 by fastforce
+  }
+  note case32 = this
+  { assume c: "is_IntVal64 xval"
+    obtain xxval where x64: "xval = IntVal64 xxval"
+      using c is_IntVal64_def by blast
+    obtain yyval where y64: "yval = IntVal64 yyval"
+      using \<open>is_IntVal64 xval = is_IntVal64 yval\<close> c is_IntVal64_def by auto
+    have xs: "\<exists> lo hi. stamp_expr x = IntegerStamp 64 lo hi"
+      by (simp add: \<open>is_IntVal64 xval \<Longrightarrow> (\<exists>lo hi. stamp_expr x = IntegerStamp 64 lo hi) \<and> (\<exists>lo hi. stamp_expr y = IntegerStamp 64 lo hi)\<close> c)
+    have ys: "\<exists> lo hi. stamp_expr y = IntegerStamp 64 lo hi"
+      using \<open>is_IntVal64 xval \<Longrightarrow> (\<exists>lo hi. stamp_expr x = IntegerStamp 64 lo hi) \<and> (\<exists>lo hi. stamp_expr y = IntegerStamp 64 lo hi)\<close> c by blast
+    have "sint yyval \<le> stpi_upper (stamp_expr y)"
+      using y64 ys yvalid by force
+    have "stpi_lower (stamp_expr x) \<le> sint xxval"
+      using x64 xs xvalid by force
+    have "stpi_upper (stamp_expr y) < stpi_lower (stamp_expr x)"
+      using assms(1) unfolding stamp_under.simps
+      by auto
+    then have "yyval <s xxval"
+      using assms(1) unfolding stamp_under.simps
+      using \<open>sint yyval \<sqsubseteq> stpi_upper (stamp_expr y)\<close> \<open>stpi_lower (stamp_expr x) \<sqsubseteq> sint xxval\<close> word_sless_alt by fastforce
+    then have "(intval_less_than xval yval) = IntVal32 0"
+      using signed.less_imp_triv x64 y64 by fastforce
+  }
+  note case64 = this
+  have "(intval_less_than xval yval) = IntVal32 0"
+    using \<open>is_IntVal32 xval \<or> is_IntVal64 xval\<close> case32 case64 by fastforce
+  then show ?thesis
+    by (metis BinaryExprE assms(2) bin_eval.simps(11) evalDet val_to_bool.simps(1) xval_def yval_def)
+qed
+
+end
